make silr val_type actually use step index as measure

dev2015/nano0-total-silr.v
@@ -156,19 +156,45 @@ Definition tevaln nm env e n1 v :=
 
 
 (* need to use Fixpoint because of positivity restriction *)
-Fixpoint val_type n v T : Prop := match v, T with
+Fixpoint val_type n v T {struct n}: Prop := match v, T with
 | vbool b, TBool => True
-| vabs env y, TFun T1 T2 =>
+| vabs env y, TFun T1 T2 =>  match n with | 0 => True | S n0 => 
   (* forall n nx, R n nx H tx vx T1 -> R (n-nx) ny (vx::vf::H) vy T2 *)
   (* NOTE: trouble b/c R does not include vx!! *)
-  forall nx vx, 
+  forall nx vx, nx <> 0 ->
+      val_type (S n0 - (S(nx-1))) vx T1 -> forall ry ny,
+      (* R nm (vx::(vabs env y)::env) y T2 *)
+      teval (n-nx) (vx::(vabs env y)::env) y = (ny, Some ry) ->
+      exists vy,
+        ny <> 0 /\ ry = Some vy /\ val_type (n0-(nx-1)-ny) vy T2
+  end                                          
+| _,_ => False
+end.
+
+(* unfolding lemma is handy, otherwise we need to destruct n.
+   we also take the opportunity to rewrite n/nx into saner form *)
+Lemma val_type_unfold: forall n v T, val_type n v T <-> match v, T with
+| vbool b, TBool => True
+| vabs env y, TFun T1 T2 =>  match n with | 0 => True | S n0 => 
+  (* forall n nx, R n nx H tx vx T1 -> R (n-nx) ny (vx::vf::H) vy T2 *)
+  (* NOTE: trouble b/c R does not include vx!! *)
+  forall nx vx, nx <> 0 ->
       val_type (n-nx) vx T1 -> forall ry ny,
       (* R nm (vx::(vabs env y)::env) y T2 *)
       teval (n-nx) (vx::(vabs env y)::env) y = (ny, Some ry) ->
       exists vy,
         ny <> 0 /\ ry = Some vy /\ val_type (n-nx-ny) vy T2
+  end                                          
 | _,_ => False
 end.
+Proof. 
+  intros. destruct n. simpl. split. eauto. eauto. 
+  simpl. destruct v; destruct T; try solve [split; eauto].
+  split. 
+  - intros. specialize (H nx vx H0). assert (n - (nx - 1) = S n -nx) as R. omega. rewrite R in H. eapply H; eauto.
+  - intros. specialize (H nx vx H0). destruct nx. destruct H0. eauto.
+    assert ((S nx - 1) = nx) as R. omega. rewrite R. eapply H. rewrite R in H1. eapply H1. eauto. 
+Qed.
 
 Definition R n H t T := 
   (* tevaln H t v /\ val_type v T. *)
@@ -200,10 +226,13 @@ Proof.
   intros.
   case_eq (eq_nat_dec j (S n)); intros E _. subst j. eauto.
   assert (val_type n v T). {
-    destruct T; destruct v; try  eauto.
-    simpl. intros. simpl in H0. specialize (H0 (S nx) vx H1 ry ny H2). eapply H0.
+    rewrite val_type_unfold. rewrite val_type_unfold in H0. 
+    destruct T; destruct v; try eauto. 
+    destruct n. eauto. intros. eapply (H0 (S nx) vx _ H2 ry ny). eauto. 
   }
-  eapply IHn. omega. eauto. 
+  eapply IHn. omega. eauto.
+Grab Existential Variables.
+  omega.
 Qed.
 
 Lemma R_down: forall n j H t T, j <= n -> R n H t T -> R j H t T.
@@ -241,10 +270,10 @@ Proof.
   inversion W; intros ? WFE.
   
   - Case "True". 
-    eexists. simpl in H2. inversion H2. repeat split; simpl; eauto.
+    eexists. simpl in H2. inversion H2. repeat split; try rewrite val_type_unfold; eauto.
 
   - Case "False".
-    eexists. simpl in H2. inversion H2. repeat split; simpl; eauto.
+    eexists. simpl in H2. inversion H2. repeat split; try rewrite val_type_unfold; eauto.
 
   - Case "Var".
     eapply WFE. eauto.
@@ -262,7 +291,7 @@ Proof.
     destruct (RF rf nf) as [vf [? [EQVF VTF]]]. eauto.
     subst rf.
     
-    simpl in VTF. destruct vf. contradiction.
+    rewrite val_type_unfold in VTF. destruct vf. contradiction.
     
 
     assert (R (n-nf) venv0 x T1) as RX. eapply IHnn. omega. eauto. eauto.
@@ -278,7 +307,9 @@ Proof.
     destruct EY as [ny [ry|]]; try solve [inversion EVY].
     inversion EVY. subst r n1. clear EVY.
 
-    specialize (VTF _ _ VTX _ _ HeqEY).
+    remember (n-nf) as nnf. destruct nnf. inversion HeqEX. rewrite Heqnnf in *. clear Heqnnf. (* can't be zero *)
+    
+    specialize (VTF _ _ H5 VTX _ _ HeqEY).
     assert ((n - nf - nx - ny = S n - S (nf + nx + ny))) as RW. omega.
     rewrite <-RW.
     destruct VTF as [? [? [? ?]]]. eexists. repeat split; eauto. 
@@ -298,11 +329,12 @@ Proof.
     assert (forall nm1, nm1 <= n -> forall nm, nm <= nm1 ->
                        val_type nm (vabs venv0 y) (TFun T1 T2)) as IND.
     intros nm1. induction nm1.
-    (* z *) simpl. intros. destruct nm. solve [inversion H9]. solve [inversion H5].
+    (* z *) simpl. intros. destruct nm. simpl. eauto. solve [inversion H5].
     (* s n *) intros ? ? ?. 
 
     (* goal val_type n (vabs venv0 y) (TFun T1 T2) *)
-    simpl. intros ? ? ?.
+    destruct nm; rewrite val_type_unfold. eauto.
+    intros ? ? ? ?.
     
     eapply IHnn. omega. eauto. 
 
@@ -313,7 +345,7 @@ Proof.
       intros ? ? IX.
       
       unfold R. intros ? ? EVX.
-      remember (nm-nx) as nx2.
+      remember (S nm-nx) as nx2.
       destruct nx2. solve [inversion EVX].
       simpl in EVX. destruct WFE as [L WX].
       simpl in IX. rewrite <-L in IX.
